small step tests

Owl/owl_typing.v
@@ -17,6 +17,14 @@ Definition lift_delta {l : nat} {d : nat} (Delta : fin (S d) -> ty l d)
   := fun i => ren_ty id shift (Delta i).
 
 Inductive is_value { l d m } : tm l d m -> Prop :=
+| error_value : is_value error
+| skip_value : is_value skip
+| loc_value : forall n,
+  is_value (loc n)
+| bitstring_value : forall b,
+  is_value (bitstring b)
+| fixlam_value : forall e,
+  is_value (fixlam e)
 | pair_value : forall v1 v2,
   is_value v1 ->
   is_value v2 ->
@@ -27,6 +35,10 @@ Inductive is_value { l d m } : tm l d m -> Prop :=
 | inr_value : forall v,
   is_value v ->
   is_value (inr v)
+| tlam_value : forall e,
+  is_value (tlam e)
+| l_lam_value : forall e,
+  is_value (l_lam e)
 | pack_value : forall v,
   is_value v ->
   is_value (pack v).
@@ -107,45 +119,128 @@ Definition test_mem (l d m : nat) : mem l d m :=
 
 Definition allocate {l d m} (location : nat) (v : tm l d m) (memory : mem l d m) : (mem l d m) :=
   fun i =>
-    if Nat.eq_dec i location
+    if (Nat.eq_dec i location)
     then Some v
     else memory i.
 
 Parameter fresh : forall {l d m}, mem l d m -> nat.
 
+Parameter valid_constraint : forall {l}, constr l -> Prop.
+
 Axiom fresh_not_allocated :
   forall {l d m} (memory : mem l d m), memory (fresh memory) = None.
 
-Inductive reduction {l d m : nat} : (tm l d m * mem l d m) -> (tm l d m * mem l d m) -> Prop := 
+Inductive reduction (l d m : nat) : (tm l d m * mem l d m) -> (tm l d m * mem l d m) -> Prop := 
 | r_zero : forall b memory, 
-  reduction (zero (bitstring b), memory) ((bitstring (generate_zero b)), memory)
+  reduction l d m (zero (bitstring b), memory) ((bitstring (generate_zero b)), memory)
 | r_ift : forall b e1 e2 memory, 
   all_zero b -> 
-  reduction (if_tm (bitstring b) e1 e2, memory) (e1, memory)
+  reduction l d m (if_tm (bitstring b) e1 e2, memory) (e1, memory)
 | r_iff : forall b e1 e2 memory, 
-  (not (all_zero b)) -> reduction (if_tm (bitstring b) e1 e2, memory) (e2, memory)
+  (not (all_zero b)) -> 
+  reduction l d m (if_tm (bitstring b) e1 e2, memory) (e2, memory)
 | r_alloc : forall v memory,
   is_value v ->
   let res := (fresh memory) in
-  reduction (alloc v, memory) (loc res, (allocate res v memory))
+  reduction l d m (alloc v, memory) (loc res, (allocate res v memory))
 | r_deref : forall n memory v,
   memory n = Some v ->
-  reduction (dealloc (loc n), memory) (v, memory)
+  reduction l d m (dealloc (loc n), memory) (v, memory)
 | r_assign : forall n v memory,
   is_value v ->
-  reduction (assign (loc n) v, memory) (skip, (allocate n v memory))
+  reduction l d m (assign (loc n) v, memory) (skip, (allocate n v memory))
 | r_fix : forall e v memory,
   is_value v ->
-  reduction (Core.app (fixlam e) v, memory) ((subst_tm var_label var_ty (scons v (scons (fixlam e) var_tm)) e), memory)
-| r_lapp : forall e l memory,
-  reduction (lapp (l_lam e) l, memory) ((subst_tm (scons l var_label) var_ty var_tm e), memory).
+  reduction l d m (Core.app (fixlam e) v, memory) ((subst_tm var_label var_ty (scons v (scons (fixlam e) var_tm)) e), memory)
+| r_pair_l : forall v1 v2 memory,
+  is_value v1 ->
+  is_value v2 ->
+  reduction l d m (left_tm (tm_pair v1 v2), memory) (v1, memory)
+| r_pair_r : forall v1 v2 memory,
+  is_value v1 ->
+  is_value v2 ->
+  reduction l d m (right_tm (tm_pair v1 v2), memory) (v2, memory)
+| r_case_l : forall v e1 e2 memory,
+  is_value v ->
+  reduction l d m (case (inl v) e1 e2, memory) (subst_tm var_label var_ty (scons v var_tm) e1, memory)
+| r_case_r : forall v e1 e2 memory,
+  is_value v ->
+  reduction l d m (case (inr v) e1 e2, memory) (subst_tm var_label var_ty (scons v var_tm) e2, memory)
+| r_tapp : forall e t memory,
+  reduction l d m (tapp (tlam e) t, memory) (subst_tm var_label (scons t var_ty) var_tm e, memory)
+| r_lapp : forall e lab memory,
+  reduction l d m (lapp (l_lam e) lab, memory) ((subst_tm (scons lab var_label) var_ty var_tm e), memory)
+| r_unpack : forall v e memory,
+  is_value v ->
+  reduction l d m (unpack (pack v) e, memory) (subst_tm var_label var_ty (scons v var_tm) e, memory)
+| r_iflt : forall c e1 e2 memory,
+  valid_constraint c ->
+  reduction l d m (if_c c e1 e2, memory) (e1, memory)
+| r_iflf : forall c e1 e2 memory,
+  not (valid_constraint c) ->
+  reduction l d m (if_c c e1 e2, memory) (e2, memory).
+
+Definition stuck { l d m } (v : tm l d m) (memory : mem l d m) :=
+  not (is_value v) /\
+      (forall v' memory',
+        not (reduction l d m (v, memory) (v', memory'))).
+
+Inductive gen_reduction {l d m : nat} : (tm l d m * mem l d m) -> (tm l d m * mem l d m) -> Prop := 
+| gr_reduce : forall v memory v' memory',
+  reduction l d m (v, memory) (v', memory') ->
+  gen_reduction (v, memory) (v', memory')
+| gr_stuck : forall v memory,
+  stuck v memory ->
+  gen_reduction (v, memory) (error, memory).
+
+Inductive step (l d m : nat) : (tm l d m * mem l d m) -> (tm l d m * mem l d m) -> Prop :=
+| step_ctx : forall K e memory e' memory',
+  gen_reduction (e, memory) (e', memory') ->
+  step l d m (Plug K e, memory) (Plug K e', memory').
+
+Lemma test_step :
+  forall memory,
+    step 0 0 0 ((zero (bitstring (bone (bone bend)))), memory) ((bitstring (bzero (bzero bend))), memory).
+Proof.
+  intros.
+  assert ((Plug (KHole 0 0 0) (zero (bitstring (bone (bone bend))))) = (zero (bitstring (bone (bone bend))))) as Ht. {
+    simpl. reflexivity.
+  }
+  rewrite <- Ht.
+  specialize (step_ctx 0 0 0 (KHole 0 0 0) (zero (bitstring (bone (bone bend)))) memory (bitstring (bzero (bzero bend))) memory) as Hn.
+  specialize (gr_reduce (zero (bitstring (bone (bone bend)))) memory (bitstring (bzero (bzero bend))) memory) as Hb.
+  specialize (r_zero 0 0 0 (bone (bone bend)) memory) as Hx.
+  specialize (Hb Hx).
+  specialize (Hn Hb).
+  assumption.
+Qed.
+
+Lemma test_error :
+  forall memory,
+    step 0 0 0 (zero skip, memory) (error, memory).
+Proof.
+  intros.
+  assert ((Plug (KHole 0 0 0) (zero skip)) = (zero skip)) as Hp. {
+    simpl. reflexivity.
+  }
+  rewrite <- Hp.
+  specialize (step_ctx 0 0 0 (KHole 0 0 0) (zero skip) memory error memory) as Hb.
+  specialize (gr_stuck (zero skip) memory) as Hx.
+  assert (stuck (zero skip) memory) as Hs. {
+    unfold stuck.
+    split.
+    - intros H. inversion H.
+    - intros. intro H. inversion H. 
+  }
+  specialize (Hx Hs).
+  specialize (Hb Hx).
+  simpl.
+  simpl in Hb.
+  assumption.
+Qed.
   
 
-Inductive step {l d m : nat} : (tm l d m * mem l d m) -> (tm l d m * mem l d m) -> Prop :=
-| step_ctx : forall K e memory e' memory',
-  reduction (e, memory) (e', memory') ->
-  step (Plug K e, memory) (Plug K e', memory').
-  
+
 (* Missing ST_VAR ST_DATA ST_LATUNIV *)
 
 Inductive subtype {l d} (Phi : phi_context l) (Delta : delta_context l d) :
